

Sub → MATHS

Module → 2

Lecture → 09

Date _____ Page _____

ex → 9

Q.1) If $z = x^y + y^n$, evaluate $\frac{\partial^2 z}{\partial y \partial x} = y x^{y-1} \log n + x^{y-1} + y^{n-1} + x y^{n-1} \cdot \log y$

Ans → $\frac{\partial z}{\partial x} = y x^{y-1} + y^n \log y$

∴ $\frac{\partial^2 z}{\partial x \partial y} = x^{y-1} + y x^{y-1} \log x + \log y \cdot n \cdot y^{n-1} + \frac{y^n}{y}$
 $= x^{y-1} + x^{y-1} \cdot \log n \cdot y + n \cdot \log y \cdot y^{n-1} + y^{n-1}$

Q.2) If $z = \tan(y+ax) + (y-ax)^{3/2}$, then show that $\frac{\partial^2 z}{\partial x^2} = a^2 \frac{\partial^2 z}{\partial y^2}$

Ans → $\frac{\partial z}{\partial x} = \sec^2(y+ax) (0+a) + \frac{3}{2} (y-ax)^{1/2} (0-a)$

$$\frac{\partial z}{\partial x} = a \cdot \sec^2(y+ax) - \frac{3a}{2} (y-ax)^{1/2}$$

∴ $\frac{\partial^2 z}{\partial x^2} = a \cdot 2 \cdot \sec(y+ax) \cdot \sec^2(y+ax) \cdot \tan(y+ax) (0+a) - \frac{3a}{2} \times \frac{1}{2} (y-ax)^{-1/2} (-a)$

∴ $\frac{\partial^2 z}{\partial x^2} = 2a^2 \cdot \sec^2(y+ax) \cdot \tan(y+ax) + \frac{3a^2}{4} (y-ax)^{-1/2}$

$$\frac{\partial z}{\partial y} = \sec^2(y+ax) + \frac{3}{2} (y-ax)^{1/2}$$

$$\frac{\partial^2 z}{\partial y^2} = 2 \sec(y+ax) \cdot \sec^2(y+ax) \cdot \tan(y+ax) + \frac{3}{2} \times \frac{1}{2} (y-ax)^{-1/2}$$

$$\therefore \frac{\partial^2 z}{\partial^2 y} = 2 \sec^2(y+ax) \cdot \tan(y+ax) + \frac{3}{4} (y-ax)^{-1/2}$$

$$\therefore a^2 \frac{\partial^2 z}{\partial^2 y} = 2a^2 \sec^2(y+ax) \cdot \tan(y+ax) + \frac{3}{4} a^2 (y-ax)^{-1/2}$$

$$\therefore \frac{\partial^2 z}{\partial^2 x^2} = a^2 \frac{\partial^2 z}{\partial^2 y^2}$$

Q.3) If $u = \log(x^3 + y^3 - x^2y - xy^2)$, then show that $\frac{\partial^2 u}{\partial x^2} + 2 \frac{\partial^2 u}{\partial x \partial y} + \frac{\partial^2 u}{\partial y^2} = -4$

Ans $\rightarrow \frac{\partial u}{\partial x} = \frac{1}{(x^3 + y^3 - x^2y - xy^2)} \times (3x^2 + 0 - 2xy - y^2)$

$$\frac{\partial u}{\partial x} = \frac{3x^2 - 2xy - y^2}{x^3 + y^3 - x^2y - xy^2}$$

$$\therefore \frac{\partial^2 u}{\partial x^2} = \frac{(x^3 + y^3 - x^2y - xy^2)(6x - 2y) - (3x^2 - 2xy - y^2)^2}{(x^3 + y^3 - x^2y - xy^2)^2}$$

$$\begin{aligned} \therefore \frac{\partial^2 u}{\partial x^2} &= \frac{6x^4 - 2x^3y + 6xy^3 - 2y^4 - 6x^3y + 2x^2y^2 - 6x^2y^2 + 2xy^3 - 9x^4}{(x^3 + y^3 - x^2y - xy^2)^2} \\ &= \frac{-3x^4 + 4x^3y + 6xy^3 - 3y^4 - 5x^2y^2}{(x^3 + y^3 - x^2y - xy^2)^2} \end{aligned}$$

$$\frac{\partial u}{\partial y} = 1/3$$

$$\frac{\partial u}{\partial x} = \frac{3x^2 - 2xy - y^2}{x^3 + y^3 - x^2y - xy^2}$$

$$\therefore \frac{\partial u}{\partial x} = \frac{3x^2 + (x-y)^2 - x^2 - y^2 - y^2}{x^3 + y^3 - x^2y - xy^2} \dots (x-y)^2 = x^2 - 2xy + y^2$$

$$\therefore -2xy = (x-y)^2 - x^2 - y^2$$

$$\therefore \frac{\partial u}{\partial x} = \frac{(x-y)^2 + 2x^2 - 2y^2}{(x-y)^3 + y^3 + 3x^2y - 3xy^2 - \dots} \left[\begin{aligned} (x-y)^3 &= x^3 - y^3 - 3x^2y + 3xy^2 \\ (x-y)^3 + y^3 + 3x^2y - 3xy^2 &= x^3 \end{aligned} \right]$$

$$\therefore \frac{\partial u}{\partial x} = \frac{(x-y)^2 + 2(x+y)(x-y)}{(x-y)^3 + 2y^3 + 2x^2y - 4xy^2}$$

$$\therefore \frac{\partial u}{\partial x} = \frac{(x-y)(x-y + 2x + 2y)}{(x-y)^3 + 2y(y^2 + x^2 - 2xy)}$$

$$\therefore \frac{\partial u}{\partial x} = \frac{(x-y)(3x+y)}{(x-y)^3 + 2y(x-y)^2}$$

$$\therefore \frac{\partial u}{\partial x} = \frac{(x-y)(3x+y)}{(x-y)^2(x-y + 2y)} = \frac{3x+y}{(x-y)(x+y)}$$

$$\therefore \boxed{\frac{\partial u}{\partial x} = \frac{3x+y}{x^2-y^2}} \dots (i)$$

$$\therefore \frac{\partial^2 u}{\partial x^2} = \frac{(x^2-y^2)(3) - (3x+y)(2x)}{(x^2-y^2)^2}$$

$$\frac{\partial^2 u}{\partial x^2} = \frac{3x^2 - 3y^2 - 6xy - 2xy}{(x^2 - y^2)^2} = \frac{-3x^2 - 3y^2 - 2xy}{(x^2 - y^2)^2}$$

form (i)

$$\frac{\partial^2 u}{\partial x \partial y} = \frac{(x^2 - y^2)(1) - (3x + y)(-2y)}{(x^2 - y^2)^2}$$

$$\therefore \frac{\partial^2 u}{\partial x \partial y} = \frac{x^2 - y^2 + 6xy + 2y^2}{(x^2 - y^2)^2} = \frac{x^2 + y^2 + 6xy}{(x^2 - y^2)^2}$$

$$\therefore u = \log(x^3 + y^3 - x^2y - xy^2)$$

$$\therefore \frac{du}{dy} = \frac{1}{(x^3 + y^3 - x^2y - xy^2)} \times (0 + 3y^2 - x^2 - 2xy)$$

$$\therefore \frac{\partial u}{\partial y} = \frac{3y^2 - x^2 - 2xy}{(x-y)^2 (x+y)}$$

→ this is same as
it had done for

$$\frac{\partial u}{\partial x}$$

$$\therefore \frac{\partial u}{\partial y} = \frac{3y^2 - x^2 + (x-y)^2 - x^2 - y^2}{(x-y)^2 (x+y)}$$

$$\therefore \frac{\partial u}{\partial y} = \frac{2y^2 - 2x^2 + (x-y)^2}{(x-y)^2 (x+y)}$$

$$\therefore \frac{\partial u}{\partial y} = \frac{-(x-y)(2y+2x+x-y)}{(x-y)^2}$$

$$\therefore \frac{\partial u}{\partial x} = \frac{2(x+y)(y-x) + (x-y)^2}{(x-y)^2(x+y)}$$

$$\frac{\partial u}{\partial y} = \frac{(x-y)^2 - 2(x+y)(x-y)}{(x-y)^2(x+y)}$$

$$\frac{\partial u}{\partial y} = \frac{x-y - 2x-2y}{x^2-y^2} = \frac{-x-3y}{x^2-y^2}$$

$$\therefore \frac{\partial^2 u}{\partial^2 y^2} = \frac{(x^2-y^2)(-3) - (-x-3y)(-2y)}{(x^2-y^2)^2}$$

$$\therefore \frac{\partial^2 u}{\partial y^2} = \frac{-3x^2+3y^2-2xy-6y^2}{(x^2-y^2)^2} = \frac{-3x^2-3y^2-2xy}{(x^2-y^2)^2}$$

$$\therefore \frac{\partial^2 u}{\partial x^2} + 2 \frac{\partial^2 u}{\partial x \partial y} + \frac{\partial^2 u}{\partial y^2} = \frac{-3x^2-3y^2-2xy}{(x^2-y^2)^2} + \frac{2(x^2+y^2+6xy)}{(x^2-y^2)^2} - \frac{3x^2-3y^2-2xy}{(x^2-y^2)^2}$$

$$\therefore = \frac{-6x^2-6y^2-4xy+2x^2+2y^2+12xy}{(x^2-y^2)^2}$$

$$= \frac{-4x^2-4y^2+8xy}{(x^2-y^2)^2} = \frac{-4(x^2+y^2-2xy)}{(x+y)^2(x-y)^2}$$

$$= \frac{-4(x-y)^2}{(x+y)^2(x-y)^2} = \frac{-4}{(x+y)^2}$$

hence proved.